src/Mman.fst
@@ -5,8 +5,10 @@ open Steel.Effect
 module A = Steel.Array
 
 module U8 = FStar.UInt8
+module U32 = FStar.UInt32
 module U64 = FStar.UInt64
 module US = FStar.SizeT
+module UP = FStar.PtrdiffT
 module AL = ArrayList
 module R = Steel.Reference
 
@@ -108,6 +110,95 @@ assume val mmap_sizes_init (len: US.t)
 
 open NullOrVarray
 
+module FML = FStar.Math.Lemmas
+
+open MiscArith
+
+open FStar.Mul
+
+#push-options "--fuel 0 --ifuel 0 --z3rlimit 100"
+let nearest_multiple_upper_rounding
+  (n: nat)
+  (multiple: nat{multiple > 0})
+  : Pure nat
+  (requires True)
+  (ensures fun r ->
+    r >= 0 /\
+    r % multiple == 0 /\
+    r >= n /\
+    r - n < multiple
+  )
+  =
+  if n % multiple <> 0
+  then (
+    let r = n - (n % multiple) + multiple in
+    FML.euclidean_division_definition n multiple;
+    assert (n - (n % multiple) == (n/multiple)*multiple);
+    lemma_mod_mul2 (n/multiple) multiple multiple;
+    assert ((n - (n % multiple)) % multiple == 0);
+    lemma_mod_plus2 (n - (n % multiple)) multiple multiple;
+    r
+  ) else n
+
+let rec nearest_multiple_upper_rounding_lemma
+  (n: nat)
+  (multiple: nat{multiple > 0})
+  (k: nat)
+  : Lemma
+  (requires k >= n /\ k % multiple == 0)
+  (ensures
+    k >= nearest_multiple_upper_rounding n multiple
+  )
+  (decreases k)
+  =
+  let n' = nearest_multiple_upper_rounding n multiple in
+  assert (n' >= n /\ n' % multiple == 0);
+  if k < n'
+  then (
+    assert (n' > n);
+    assert (n % multiple <> 0);
+    let diff = n' - k in
+    assert (0 < diff);
+    assert (n' % multiple == 0);
+    assert (k % multiple == 0);
+    lemma_mod_add_inv k multiple;
+    assert ((-k) % multiple == 0);
+    lemma_mod_plus2 (-k) n' multiple;
+    assert (diff % multiple == 0);
+    assert (diff >= multiple);
+    if diff >= multiple
+    then nearest_multiple_upper_rounding_lemma n multiple (k - multiple)
+    else ()
+ ) else ()
+
+noextract
+let spec_mmap_actual_size (size: nat)
+  : Pure nat
+  (requires True)
+  (ensures fun r ->
+    r >= 0 /\
+    r % (U32.v page_size) == 0 /\
+    r >= size /\
+    r - size < (U32.v page_size)
+  )
+  =
+  nearest_multiple_upper_rounding size (U32.v page_size)
+
+let mmap_actual_size (size: US.t)
+  : Pure US.t
+  (requires
+    US.fits (US.v size + U32.v page_size)
+  )
+  (ensures fun r ->
+    US.v r == spec_mmap_actual_size (US.v size)
+  )
+  =
+  let rem = US.rem size (u32_to_sz page_size) in
+  if rem <> 0sz
+  then US.add (US.sub size rem) (u32_to_sz page_size)
+  else size
+#pop-options
+
 // POSIX spec: mmap returns a page-aligned array of bytes;
 // thus, mmap_u8 returns a page-aligned array of bytes;
 // hence the postcondition array_u8_alignment page_size
@@ -115,19 +206,47 @@ open NullOrVarray
 assume val mmap_u8
   (size: US.t)
   : Steel (array U8.t)
-    emp
-    (fun ptr -> null_or_varray ptr)
-    (requires fun _ -> US.v size > 0)
-    (ensures fun _ ptr h1 ->
-      let s : t_of (null_or_varray ptr)
-        = h1 (null_or_varray ptr) in
-      not (A.is_null ptr) ==> (
-        A.length ptr == US.v size /\
-        A.is_full_array ptr /\
-        array_u8_alignment ptr page_size /\
-        zf_u8 s
-      )
+  emp
+  (fun ptr -> null_or_varray ptr)
+  (requires fun _ -> US.v size > 0)
+  (ensures fun _ ptr h1 ->
+    let s : t_of (null_or_varray ptr)
+      = h1 (null_or_varray ptr) in
+    not (A.is_null ptr) ==> (
+      A.length ptr == spec_mmap_actual_size (US.v size) /\
+      A.is_full_array ptr /\
+      array_u8_alignment ptr page_size /\
+      zf_u8 s
     )
+  )
+
+//open PtrdiffWrapper
+//
+//let mmap_u8_wrapper
+//  (size: US.t)
+//  : Steel (array U8.t)
+//  emp
+//  (fun ptr -> null_or_varray ptr)
+//  (requires fun _ -> US.v size > 0)
+//  (ensures fun _ ptr h1 ->
+//    let s : t_of (null_or_varray ptr)
+//      = h1 (null_or_varray ptr) in
+//    not (A.is_null ptr) ==> (
+//      A.length ptr == spec_mmap_actual_size (US.v size) /\
+//      A.length ptr <= US.v mmap_bound /\
+//      A.is_full_array ptr /\
+//      array_u8_alignment ptr page_size /\
+//      zf_u8 s
+//    )
+//  )
+//  =
+//  if US.lte size mmap_bound
+//  then (
+//    mmap_u8 size
+//  ) else (
+//    intro_null_null_or_varray #U8.t
+//  )
+
 
 // TODO: should the underlying munmap fail in a stricter manner?
 //noextract
