lib_misc/PtrdiffWrapper.fsti
@@ -1,0 +1,40 @@
+module PtrdiffWrapper
+
+module U32 = FStar.UInt32
+module US = FStar.SizeT
+module UP = FStar.PtrdiffT
+
+open FStar.Mul
+open Config
+
+// conservative axiomatization, C23 changed guarantees about ptrdiff_t bit width
+// this is an assume val
+val ptrdiff_max: v:UP.t{
+  UP.v v >= pow2 16 - 1 /\
+  (exists (k:nat). UP.v v = pow2 k - 1)
+}
+
+open MiscArith
+
+let mmap_bound : v:US.t{
+  US.fits (US.v v + 2) /\
+  US.fits (US.v v + U32.v page_size) /\
+  US.v v % U32.v page_size = 0
+}
+  =
+  let ptrdiff_max_as_sizet = UP.ptrdifft_to_sizet ptrdiff_max in
+  // US.fits(x) where x = 2^n-1
+  // y = x/2 = (2^n-1)/2 = 2^{n-1}-1
+  let r = US.add (US.div ptrdiff_max_as_sizet 2sz) 1sz in
+  eliminate exists (k:nat). UP.v ptrdiff_max = pow2 k - 1
+    returns (US.v r % U32.v page_size = 0)
+    with _. (
+      assert (UP.v ptrdiff_max == pow2 k - 1);
+      assert (US.v r == pow2 (k-1));
+      assert (U32.v page_size == pow2 12);
+      pow2_is_increasing 12 (k-1);
+      pow2_mod 12 (k-1);
+      ()
+  );
+  r
+  //normalize_term r
