src/SlabsCommon.fsti
@@ -29,18 +29,6 @@ open SlotsAlloc
 open SteelStarSeqUtils
 open FStar.Mul
 
-// TODO: to be removed/move apart ; use stdlib
-// discussion
-inline_for_extraction noextract
-let u32_to_sz
-  (x:U32.t)
-  : Tot (y:US.t{US.v y == U32.v x})
-  //: Pure US.t
-  //(requires True)
-  //(ensures fun y -> US.v y == U32.v x)
-  =
-  US.uint32_to_sizet x
-
 inline_for_extraction noextract
 let halfp = Steel.FractionalPermission.half_perm Steel.FractionalPermission.full_perm
 
